Finished main Bit-Aligned to Byte-Aligned Monad conversion lemmas.

src/Narcissus/BinLib/AlignedMonads.v
@@ -17,10 +17,10 @@ Section AlignedDecodeM.
   Definition AlignedDecodeM
              (A : Set)
              (n : nat):=
-    Vector.t char n
-    -> nat
-    -> CacheDecode
-    -> option (A * nat * CacheDecode).
+    Vector.t char n (* Vector of bytes that is being decoded *)
+    -> nat          (* The current vector index *)
+    -> CacheDecode  (* The current environment *)
+    -> option (A * nat * CacheDecode) (* Error monad + value + updated index + updated cache *).
 
   Definition BindAlignedDecodeM
              {A B : Set}
@@ -147,12 +147,16 @@ Section AlignedDecodeM.
               /\
               (forall c bs' cd',
                   f (build_aligned_ByteString v) cd = Some (c, bs', cd') ->
-                  f' v 0 cd = Some (c, n - (numBytes bs'), cd')))
-       /\ (forall n m o (v : Vector.t (word 8) (n + (m + o))) cd c cd' H,
-              f' v n cd = Some (c, o, cd') ->
-              f (build_aligned_ByteString (snd (Vector_split n (m + o) v))) cd =
-              Some (c, build_aligned_ByteString (snd (Vector_split (n + m) o (eq_rect _ _ v _ H))), cd')
-          ).
+                  f' v 0 cd = Some (c, n - (numBytes bs'), cd')
+                  /\ exists v' : Vector.t _ (n - (numBytes bs')),
+                    (build_aligned_ByteString v) = ByteString_enqueue_ByteString (build_aligned_ByteString v') bs'
+                                                                                 ))
+              (*       /\ (forall n (v : Vector.t (word 8) n) cd c n' cd', *)
+              (* f' v 0 cd = Some (c, n', cd') -> *)
+              (* exists m', *)
+              (*   {H : n = n' + m' & *)
+              (*        f (build_aligned_ByteString v) cd = *)
+              (*        Some (c, build_aligned_ByteString (snd (Vector_split _ _ (eq_rect _ _ v _ H))), cd')}) *).
 
   Lemma DecodeMEquivAlignedDecodeM_trans  {C} :
     forall bit_decoder1 byte_decoder1 bit_decoder2 byte_decoder2,
@@ -163,10 +167,11 @@ Section AlignedDecodeM.
   Proof.
     unfold DecodeMEquivAlignedDecodeM; intros; intuition; rewrite <- ?H0, <- ?H1; eauto.
     - eapply H; rewrite H0; eauto.
-    - eapply H3; rewrite H0; eauto.
-    - eapply H3; rewrite H1; eauto.
-    - eapply H3; rewrite H0; eauto.
-    - eapply H5; rewrite H1; eauto.
+    - eapply H4; rewrite H0; eauto.
+    - eapply H4; rewrite H1; eauto.
+    - eapply H4; rewrite H0; eauto.
+    - rewrite <- H0 in H3; apply H4 in H3; destruct H3 as [? [? ?] ];
+      eauto.
   Qed.
 
   Lemma Return_DecodeMEquivAlignedDecodeM {A : Set}
@@ -181,9 +186,136 @@ Section AlignedDecodeM.
     - discriminate.
     - unfold ReturnAlignedDecodeM, numBytes; injections.
       simpl; repeat f_equal; omega.
-    - unfold ReturnAlignedDecodeM in H0; injections; simpl.
-      repeat f_equal.
-  Admitted.
+    - unfold ReturnAlignedDecodeM in H; injections.
+      assert ((n - numBytes (build_aligned_ByteString v)) = 0)
+             by (unfold numBytes; simpl; omega).
+      rewrite H.
+      setoid_rewrite <- build_aligned_ByteString_append.
+      simpl; eexists (@Vector.nil _); reflexivity.
+  Qed.
+
+  Lemma A_decode_aligned_shift {A : Set}
+        (A_decode_aligned : forall {numBytes}, AlignedDecodeM A numBytes)
+    : (forall (numBytes_hd n : nat) (v : Vector.t char (S numBytes_hd)) (cd : CacheDecode),
+          @A_decode_aligned (S numBytes_hd) v (S n) cd =
+          (Ifopt @A_decode_aligned numBytes_hd (Vector.tl v) n cd as a0
+        Then Some (fst (fst a0), S (snd (fst a0)), snd a0) Else None))
+      -> forall (numBytes_hd numBytes_tl : nat)
+                (v : Vector.t char (numBytes_hd + numBytes_tl)) (cd : CacheDecode),
+          @A_decode_aligned _ v numBytes_hd cd =
+          (Ifopt @A_decode_aligned _ (snd (Vector_split _ _ v)) 0 cd as a0
+        Then Some (fst (fst a0), numBytes_hd + (snd (fst a0)), snd a0) Else None).
+  Proof.
+    induction numBytes_hd; simpl; intros.
+    - destruct ( A_decode_aligned numBytes_tl v 0 cd) as [ [ [? ?] ?]  | ]; reflexivity.
+    - rewrite H.
+      rewrite IHnumBytes_hd; destruct (Vector_split numBytes_hd numBytes_tl (Vector.tl v)) eqn: ?; simpl.
+      match goal with
+        |- context [Vector_split ?m ?n ?v] => replace (Vector_split m n v) with (t, t0)
+      end; simpl.
+      destruct (A_decode_aligned numBytes_tl t0 0 cd); simpl; reflexivity.
+      rewrite <- Heqp;  reflexivity.
+  Qed.
+
+  (* Lemma A_decode_aligned_shift' {A : Set}
+        (A_decode_aligned : forall {numBytes}, AlignedDecodeM A numBytes)
+    : (forall (numBytes_hd n : nat) (v : Vector.t char (S numBytes_hd)) (cd : CacheDecode),
+          @A_decode_aligned (S numBytes_hd) v (S n) cd =
+          (Ifopt @A_decode_aligned numBytes_hd (Vector.tl v) n cd as a0
+        Then Some (fst (fst a0), S (snd (fst a0)), snd a0) Else None))
+      -> forall (numBytes_hd numBytes_tl : nat)
+                (v : Vector.t char (numBytes_hd + numBytes_tl)) (cd : CacheDecode),
+        @A_decode_aligned _ (snd (Vector_split _ _ v)) 0 cd =
+          (Ifopt @A_decode_aligned _ v numBytes_hd cd as a0
+        Then Some (fst (fst a0), (snd (fst a0)) - numBytes_hd, snd a0) Else None).
+  Proof.
+    induction numBytes_hd; simpl; intros.
+    - destruct ( A_decode_aligned numBytes_tl v 0 cd) as [ [ [? ?] ?]  | ]; simpl; eauto.
+      rewrite <- minus_n_O; reflexivity.
+    - rewrite H.
+      destruct (Vector_split numBytes_hd numBytes_tl (Vector.tl v)) eqn: ?; simpl.
+      match goal with
+        |- context [Vector_split ?m ?n ?v] => replace (Vector_split m n v) with (t, t0)
+      end; simpl.
+      destruct (A_decode_aligned (numBytes_hd + numBytes_tl) (Vector.tl v) numBytes_hd cd) as [ [ [? ?] ?] | ]
+                                                                                                eqn: ?; simpl.
+      specialize (IHnumBytes_hd _ (Vector.append
+                                     (fst (Vector_split numBytes_hd numBytes_tl (Vector.tl v)))
+                                     (snd (Vector_split numBytes_hd numBytes_tl (Vector.tl v)))) cd);
+        simpl in *.
+      rewrite Heqp in IHnumBytes_hd; simpl in *.
+      replace (snd (Vector_split numBytes_hd numBytes_tl (Vector.append t t0))) with
+          t0 in IHnumBytes_hd.
+      + rewrite IHnumBytes_hd.
+      destruct (A_decode_aligned numBytes_tl t0 0 cd); simpl; reflexivity.
+      rewrite <- Heqp;  reflexivity.
+  Qed. *)
+
+  Lemma proper_consumer_t_None {C}
+        (t' : forall {numBytes}, AlignedDecodeM C numBytes)
+        (t'_OK : forall (numBytes_hd n0 : nat) (v0 : Vector.t char (S numBytes_hd)) (cd0 : CacheDecode),
+            @t' (S numBytes_hd) v0 (S n0) cd0 =
+            (Ifopt @t' numBytes_hd (Vector.tl v0) n0 cd0 as a0 Then
+        Some (fst (fst a0), S (snd (fst a0)), snd a0) Else None))
+    : forall {n m} (v : Vector.t (word 8) (m + n)) (v1 : Vector.t char m) (v2 : Vector.t char n) cd,
+      t' v2 0 cd = None ->
+      build_aligned_ByteString v = build_aligned_ByteString (Vector.append v1 v2)  ->
+      t' v m cd = None.
+  Proof.
+    intros.
+    apply build_aligned_ByteString_inj in H0; subst.
+    revert n v2 cd H; induction v1.
+    - simpl; intros; eauto.
+    - simpl; intros.
+      rewrite t'_OK.
+      eapply IHv1 in H.
+      simpl; rewrite H; reflexivity.
+  Qed.
+
+  Lemma proper_consumer_t_None' {C}
+        (t' : forall {numBytes}, AlignedDecodeM C numBytes)
+        (t'_OK : forall (numBytes_hd n0 : nat) (v0 : Vector.t char (S numBytes_hd)) (cd0 : CacheDecode),
+            @t' (S numBytes_hd) v0 (S n0) cd0 =
+            (Ifopt @t' numBytes_hd (Vector.tl v0) n0 cd0 as a0 Then
+        Some (fst (fst a0), S (snd (fst a0)), snd a0) Else None))
+    : forall {n m} (v : Vector.t (word 8) (m + n)) (v1 : Vector.t char m) (v2 : Vector.t char n) cd,
+      t' v m cd = None ->
+      build_aligned_ByteString v = build_aligned_ByteString (Vector.append v1 v2) ->
+      t' v2 0 cd = None.
+
+  Proof.
+    intros.
+    apply build_aligned_ByteString_inj in H0; subst.
+    revert n v2 cd H; induction v1.
+    - simpl; intros; eauto.
+    - simpl; intros.
+      rewrite t'_OK in H.
+      eapply IHv1.
+      simpl in *;
+        destruct (t' (n + n0) (Vector.append v1 v2) n cd)
+        as [ [ [? ?] ?] | ]; simpl in *; eauto; discriminate.
+  Qed.
+
+  Lemma proper_consumer_t_Some {C}
+        (t' : forall {numBytes}, AlignedDecodeM C numBytes)
+        (t'_OK : forall (numBytes_hd n0 : nat) (v0 : Vector.t char (S numBytes_hd)) (cd0 : CacheDecode),
+            @t' (S numBytes_hd) v0 (S n0) cd0 =
+            (Ifopt @t' numBytes_hd (Vector.tl v0) n0 cd0 as a0 Then
+        Some (fst (fst a0), S (snd (fst a0)), snd a0) Else None))
+    : forall {n m} (v : Vector.t (word 8) (m + n)) (v1 : Vector.t char m) (v2 : Vector.t char n) cd c k cd',
+      t' v2 0 cd = Some (c, k, cd')
+      -> build_aligned_ByteString v = build_aligned_ByteString (Vector.append v1 v2)
+      -> t' v m cd = Some (c, m + k, cd').
+  Proof.
+    intros.
+    apply build_aligned_ByteString_inj in H0; subst.
+    revert n v2 cd H; induction v1.
+    - simpl; intros; eauto.
+    - simpl; intros.
+      rewrite t'_OK.
+      eapply IHv1 in H.
+      simpl; rewrite H; reflexivity.
+  Qed.
 
   Lemma Bind_DecodeMEquivAlignedDecodeM {A C : Set}
         (A_decode : DecodeM A ByteString)
@@ -203,26 +335,169 @@ Section AlignedDecodeM.
       destruct (A_decode_aligned numBytes_hd (Vector.tl v) n cd) as [ [ [? ?] ?] | ]; simpl.
       + specialize (H0 a); intuition.
       + reflexivity.
-    - eapply DecodeBindOpt2_inv in H3; destruct_ex; intuition.
+    - eapply DecodeBindOpt2_inv in H2; destruct_ex; intuition.
       specialize (H0 x); intuition.
-      eapply H in H5.
-      symmetry in H6; eapply H0 in H6; omega.
+      eapply H in H4.
+      symmetry in H5; eapply H0 in H5; omega.
     - destruct (A_decode (build_aligned_ByteString v) cd) as [ [ [? ?] ?] | ] eqn: ?;
         simpl in *; try discriminate.
+      assert (numBytes b <= n)%nat as nb_le_n.
+      { eapply H in Heqo.
+        unfold build_aligned_ByteString, length_ByteString in Heqo; simpl in Heqo;
+          omega. }
       unfold BindAlignedDecodeM.
-      apply H2 in Heqo; destruct_ex; intuition; subst.
-      rewrite Heqo; simpl; eauto.
-      admit.
-      unfold BindAlignedDecodeM; eapply H2 in Heqo; rewrite Heqo; reflexivity.
-    - admit.
-    - eapply DecodeBindOpt2_inv in H3; destruct_ex; intuition.
-      eapply H2 in H5.
-      unfold BindAlignedDecodeM; rewrite H5; simpl.
-      symmetry in H6.
+      apply H3 in Heqo; destruct_ex; intuition; subst; destruct_ex.
+      rewrite H4; simpl; eauto.
+      specialize (H0 a); intuition.
+      generalize (build_aligned_ByteString_split' _ _ _ H5); intros; destruct_ex.
+      rewrite H7 in *.
+      apply H8 in H2.
+      assert ((n - (n - numBytes b)) = numBytes b).
+      {rewrite sub_plus; try omega.
+       rewrite H7; auto.
+      }
+      pose proof (fun v => proper_consumer_t_None (m := n - numBytes b) (t' a) H6 v x _ _ H2).
+      assert (forall v0 : Vector.t (word 8) n,
+        build_aligned_ByteString v0 = build_aligned_ByteString (Vector.append x x0) ->
+        t' a n v0 (n - numBytes b) c = None).
+      { revert H10; clear; intro.
+        assert (n = n - numBytes b + (n - (n - numBytes b))) by omega.
+        intros.
+        specialize (H10 (eq_rect _ _ v0 _ H)).
+        destruct H.
+        eapply H10.
+        apply H0.
+      }
+      replace (n - numBytes (build_aligned_ByteString x0)) with
+          (n - numBytes b) by
+          (unfold numBytes at 2; simpl; clear; omega).
+      apply H11.
+      rewrite H5.
+      rewrite build_aligned_ByteString_append; f_equal; assumption.
+      unfold BindAlignedDecodeM; apply H3 in Heqo; rewrite Heqo; reflexivity.
+    - unfold BindAlignedDecodeM in H2.
+      destruct (A_decode (build_aligned_ByteString v) cd) as [ [ [? ?] ?] | ] eqn: ? ;
+        simpl in *; try eauto.
+      assert (numBytes b <= n)%nat as nb_le_n.
+      { eapply H in Heqo.
+        unfold build_aligned_ByteString, length_ByteString in Heqo; simpl in Heqo;
+          omega. }
+      apply H3 in Heqo; destruct_ex; intuition; subst; destruct_ex.
+      rewrite H4 in H2; simpl in H2; eauto.
+      specialize (H0 a); intuition.
+      generalize (build_aligned_ByteString_split' _ _ _ H5); intros; destruct_ex.
+      rewrite H7 in *.
+      apply H8.
+      assert ((n - (n - numBytes b)) = numBytes b).
+      {rewrite sub_plus; try omega.
+       rewrite H7; auto.
+      }
+      assert (n = n - numBytes b + (n - (n - numBytes b))) by omega.
+      eapply proper_consumer_t_None' with (v1 := x) (v0 := (eq_rect _ _ v _ H10)); eauto.
+      revert H2; clear.
+      destruct H10; simpl; intros.
+      rewrite <- H2; f_equal; omega.
+      revert H5 H7; clear; destruct H10; simpl; intros.
+      rewrite H5, build_aligned_ByteString_append; f_equal; assumption.
+    - eapply DecodeBindOpt2_inv in H2; destruct_ex; intuition.
+      assert (numBytes x0 <= n)%nat as nb_le_n.
+      { eapply H in H4.
+        unfold build_aligned_ByteString, length_ByteString in H4; simpl in H4;
+          omega. }
+      assert (numBytes bs' <= numBytes x0)%nat as nbs_le_x0.
+      { symmetry in H5.
+        eapply H0 in H5.
+        eapply H3 in H4; intuition; destruct_ex.
+        generalize (build_aligned_ByteString_split' _ _ _ H4); intros; destruct_ex.
+        rewrite H6 in H5.
+        unfold length_ByteString in H5; simpl in H5.
+        replace (n - (n - numBytes x0)) with (numBytes x0) in H5
+          by (revert nb_le_n; clear; intro; omega).
+        omega. }
+      assert (numBytes bs' <= n)%nat as nbs_le_n.
+      { etransitivity.
+        apply nbs_le_x0.
+        apply nb_le_n.
+      }
+      eapply H3 in H4.
+      intuition.
+      unfold BindAlignedDecodeM; rewrite H2; simpl; destruct_ex;
+        intuition.
+      symmetry in H5.
       specialize (H0 x); intuition.
-      admit.
-    - admit.
+      generalize (build_aligned_ByteString_split' _ _ _ H4); intros; destruct_ex.
+      rewrite H7 in *|-*.
+      eapply H8 in H5; intuition.
+      unfold numBytes at 1; simpl.
+      destruct_ex; intuition.
+      assert (n = n - numBytes x0 + (n - (n - numBytes x0))) by omega.
+      pose proof (proper_consumer_t_Some _ H6 (eq_rect _ _ v _ H10) x2 x3 _ _ _ _ H9).
+      destruct H10.
+      simpl in H11.
+      assert (n >= numBytes x0)%nat by
+          (rewrite H7; omega).
+      replace (n - (n - numBytes x0)) with (numBytes x0) by omega.
+      rewrite H11.
+      f_equal; f_equal; f_equal.
+      assert (numBytes x0 >= numBytes bs')%nat.
+      rewrite H7; omega.
+      omega.
+      rewrite H4.
+      rewrite build_aligned_ByteString_append; f_equal; eauto.
+    - eapply DecodeBindOpt2_inv in H2; destruct_ex; intuition.
+      assert (numBytes x0 <= n)%nat as nb_le_n.
+      { eapply H in H4.
+        unfold build_aligned_ByteString, length_ByteString in H4; simpl in H4;
+          omega. }
+      assert (numBytes bs' <= n)%nat as nbs_le_n.
+      { symmetry in H5.
+        eapply H0 in H5.
+        eapply H3 in H4; intuition; destruct_ex.
+        generalize (build_aligned_ByteString_split' _ _ _ H4); intros; destruct_ex.
+        etransitivity.
+        2: apply nb_le_n.
+        rewrite H6 in H5.
+        unfold length_ByteString in H5; simpl in H5.
+        replace (n - (n - numBytes x0)) with (numBytes x0) in H5
+          by (revert nb_le_n; clear; intro; omega).
+        omega. }
+      eapply H3 in H4; intuition; destruct_ex.
+      setoid_rewrite H4.
+      eapply build_aligned_ByteString_split' in H4; destruct_ex.
+      rewrite H4 in *.
+      symmetry in H5.
+      eapply H0 in H5; intuition; destruct_ex.
+      rewrite H5 in H4.
+      assert ((n - numBytes x0 + (n - (n - numBytes x0) - numBytes bs')) =
+              n - numBytes bs').
+      { assert (n >= numBytes x0)%nat by
+            (rewrite H4; rewrite H5 in nb_le_n; omega).
+        replace (n - (n - numBytes x0)) with (numBytes x0).
+        assert (numBytes x0 >= numBytes bs')%nat.
+        { rewrite H4.
+          generalize (build_aligned_ByteString_split' _ _ _ H5); intros; destruct_ex.
+          replace (ByteString_enqueue_ByteString (build_aligned_ByteString x4) bs') with
+              (build_aligned_ByteString (Vector.append x4 x5)).
+          generalize x4 x5 H8; clear.
+          generalize (n - (n - numBytes x0) - numBytes bs').
+          intro.
+          generalize (n - (n - numBytes x0) - n0); intros.
+          rewrite H8.
+          unfold numBytes; simpl; omega.
+          rewrite build_aligned_ByteString_append; f_equal; eauto.
+        }
+        omega.
+        omega.
+      }
+      generalize H7 H4; clear; intros.
+      rewrite <- H7.
+      eexists (Vector.append x2 x4).
+      rewrite build_aligned_ByteString_append.
+      rewrite <- ByteString_enqueue_ByteString_assoc.
+      rewrite <- H4; reflexivity.
   Qed.
+
+  Print Assumptions Bind_DecodeMEquivAlignedDecodeM.
 
 End AlignedDecodeM.
 
